src/lib/communication/DY.Lib.Communication.Printing.fst
@@ -113,9 +113,9 @@ let com_reqres_event_to_string #a payload_to_string =
       Some (Printf.sprintf "CommServerReceiveRequest server = %s, request = (%s), key = %s"
         server (payload_to_string request) (bytes_to_string key))
     )
-    | CommServerSendResponse server request response -> (
-      Some (Printf.sprintf "CommServerSendResponse server = %s, request = %s, response = (%s)"
-        server (payload_to_string request) (payload_to_string response))
+    | CommServerSendResponse server request response key -> (
+      Some (Printf.sprintf "CommServerSendResponse server = %s, request = %s, response = (%s), key = %s"
+        server (payload_to_string request) (payload_to_string response) (bytes_to_string key))
     )
     | CommClientReceiveResponse client server response key -> (
       Some (Printf.sprintf "CommClientReceiveResponse client = %s, server = %s, response = (%s), key = %s" 
